src/Arithmetic/DettmanMultiplication.v
@@ -2,6 +2,7 @@ Require Import Crypto.Arithmetic.Core.
 Require Import Coq.ZArith.ZArith Coq.micromega.Lia.
 Require Import Coq.Lists.List.
 Require Import Crypto.Arithmetic.ModOps.
+Require Import Crypto.Util.LetIn.
 Require Import Coq.QArith.QArith_base Coq.QArith.Qround.
 Local Open Scope list_scope.
 
@@ -13,376 +14,481 @@ Local Coercion Z.of_nat : nat >-> Z.
 Module DettmanMultiplication.
   Section DettmanMultiplication.
     Context
-        (s : Z)
-        (c' : Z)
-        (register_width : nat)
-        (n : nat)
-        (last_reduction : nat) (* should be between 1 and n - 3, inclusive.
-                                  This is the position that the final modular reduction lands in.
-                                  Larger values correspond to a faster algorithm but looser bounds on the output.
-                                *)
-        (weight: nat -> Z)
-        (p_nz' : s - c' <> 0)
-        (n_gteq_4 : (4 <= n)%nat) (* Technically we only need 2 <= n to get the proof to go through, but it doesn't make much sense to try to do this with less than four limbs.
-                                           Note that having 4 limbs corresponds to zero iterations of the "loop" function defined below. *)
+      (s : Z)
+      (c' : Z)
+      (register_width : nat)
+      (n : nat)
+      (last_reduction : nat) (* should be between 1 and n - 3, inclusive.
+                                This is the position that the final modular reduction lands in.
+                                Larger values correspond to a faster algorithm but looser bounds on the output.
+                              *)
+      (weight: nat -> Z)
+      (p_nz' : s - c' <> 0)
+      (n_gteq_4 : (4 <= n)%nat) (* Technically we only need 2 <= n to get the proof to go through, but i0..0
+0t doesn't make much sense to try to do this with less than four limbs.
+                                   Note that having 4 limbs corresponds to zero iterations of the "loop" function defined below. *)
+      (wprops : @weight_properties weight)
+        
+      (weight_0 := weight_0 wprops)
+      (weight_positive := weight_positive wprops)
+      (weight_multiples := weight_multiples wprops)
+      (weight_divides := weight_divides wprops).
+
+    Section WithoutADK.
+      Context
         (s_small : forall i: nat, (weight (i + n)%nat / weight i) mod s = 0)
         (s_big : weight (n - 1)%nat <= s)
-        (weight_lt_width : forall i: nat, (weight i * 2^register_width) mod weight (i + 1)%nat = 0)
-        (wprops : @weight_properties weight)
-        
-        (weight_0 := weight_0 wprops)
-        (weight_positive := weight_positive wprops)
-        (weight_multiples := weight_multiples wprops)
-        (weight_divides := weight_divides wprops).
-
-    (* Proofs will go through regardless of which encoding we choose for c.
-       We choose this encoding (with the weights given by the weight function)
-       so that our reductions land in the weights given by the weight function.
-       (Note that this won't necessarily work out nicely if we have a fractional
-       limbwidth.)
-     *)
-    Definition c := Positional.to_associational weight n
-                      (Positional.simple_encode weight n c').
+        (weight_lt_width : forall i: nat, (weight i * 2^register_width) mod weight (i + 1)%nat = 0).
       
-    Lemma s_positive : s > 0.
-    Proof. remember (weight_positive (n - 1)). lia. Qed.
+      (* Proofs will go through regardless of which encoding we choose for c.
+         We choose this encoding (with the weights given by the weight function)
+         so that our reductions land in the weights given by the weight function.
+         (Note that this won't necessarily work out nicely if we have a fractional
+         limbwidth.)
+       *)
+      Definition c := Positional.to_associational weight n
+                        (Positional.simple_encode weight n c').
 
-    Lemma s_nz : s <> 0.
-    Proof. remember s_positive. lia. Qed.
+      Lemma s_positive : s > 0.
+      Proof. remember (weight_positive (n - 1)). lia. Qed.
 
-    Lemma weight_nz : forall i, weight i <> 0.
-    Proof. intros i. remember (weight_positive i). lia. Qed.
+      Lemma s_nz : s <> 0.
+      Proof. remember s_positive. lia. Qed.
 
-    Lemma div_mul_le : forall x y, y > 0 -> x / y * y <= x.
-    Proof. intros x y H. remember (Zmod_eq x y H). remember (Z_mod_lt x y H). lia. Qed.
+      Lemma weight_nz : forall i, weight i <> 0.
+      Proof. intros i. remember (weight_positive i). lia. Qed.
 
-    Lemma div_nz a b : b > 0 -> b <= a -> a / b <> 0.
-    Proof. Z.div_mod_to_equations. lia. Qed.
+      Lemma div_mul_le : forall x y, y > 0 -> x / y * y <= x.
+      Proof. intros x y H. remember (Zmod_eq x y H). remember (Z_mod_lt x y H). lia. Qed.
 
-    Lemma weight_div_nz : forall i j : nat, (i <= j)%nat -> weight j / weight i <> 0.
-    Proof.
-      intros i j H. assert (0 < weight j / weight i); try lia.
-      apply Weight.weight_divides_full; assumption.
-    Qed.
+      Lemma div_nz a b : b > 0 -> b <= a -> a / b <> 0.
+      Proof. Z.div_mod_to_equations. lia. Qed.
 
-    Lemma s_small' (i j : nat) :
-      (j = i + n)%nat ->
-      weight j / weight i mod s = 0.
-    Proof. intros H. subst. apply s_small. Qed.
+      Lemma weight_div_nz : forall i j : nat, (i <= j)%nat -> weight j / weight i <> 0.
+      Proof.
+        intros i j H. assert (0 < weight j / weight i); try lia.
+        apply Weight.weight_divides_full; assumption.
+      Qed.
 
-    Lemma s_big' : s / weight (n - 1) <> 0.
-    Proof. remember (weight_positive (n - 1)). apply div_nz; lia. Qed.
+      Lemma s_small' (i j : nat) :
+        (j = i + n)%nat ->
+        weight j / weight i mod s = 0.
+      Proof. intros H. subst. apply s_small. Qed.
 
-    Lemma weight_increasing : forall i j : nat, (i <= j)%nat -> weight i <= weight j.
-    Proof.
-      intros i j H.
-      assert (0 < weight j / weight i). { apply Weight.weight_divides_full; try assumption. }
-      assert (1 <= weight j / weight i) by lia.
-      assert (1 * weight i <= weight j / weight i * weight i).
-      { apply Zmult_le_compat_r; try lia. remember (weight_positive i). lia. }
-      apply (Z.le_trans _ (weight j / weight i * weight i) _); try lia.
-      apply div_mul_le. remember (weight_positive i). lia.
-    Qed.
+      Lemma s_big' : s / weight (n - 1) <> 0.
+      Proof. remember (weight_positive (n - 1)). apply div_nz; lia. Qed.
 
-    Lemma mod_quotient_zero : forall x y, 0 < y -> x mod y = 0 -> x mod (x / y) = 0.
-    Proof.
-      intros x y H H1. rewrite Divide.Z.mod_divide_full in H1. destruct H1 as [z H1].
-      subst. rewrite Z_div_mult by lia. rewrite Z.mul_comm. apply Z_mod_mult.
-    Qed.
-    
-    Lemma weight_mod_quotient_zero : forall i j : nat,
+      Lemma weight_increasing : forall i j : nat, (i <= j)%nat -> weight i <= weight j.
+      Proof.
+        intros i j H.
+        assert (0 < weight j / weight i). { apply Weight.weight_divides_full; try assumption. }
+        assert (1 <= weight j / weight i) by lia.
+        assert (1 * weight i <= weight j / weight i * weight i).
+        { apply Zmult_le_compat_r; try lia. remember (weight_positive i). lia. }
+        apply (Z.le_trans _ (weight j / weight i * weight i) _); try lia.
+        apply div_mul_le. remember (weight_positive i). lia.
+      Qed.
+
+      Lemma mod_quotient_zero : forall x y, 0 < y -> x mod y = 0 -> x mod (x / y) = 0.
+      Proof.
+        intros x y H H1. rewrite Divide.Z.mod_divide_full in H1. destruct H1 as [z H1].
+        subst. rewrite Z_div_mult by lia. rewrite Z.mul_comm. apply Z_mod_mult.
+      Qed.
+
+      Lemma weight_mod_quotient_zero : forall i j : nat,
+          (i <= j)%nat ->
+          (weight j) mod (weight j / weight i) = 0.
+      Proof.
+        intros i j H. apply mod_quotient_zero; try apply weight_positive.
+        apply Weight.weight_multiples_full; assumption.
+      Qed.
+
+      Lemma divisible_implies_nonzero a b : 
+        a mod b = 0 ->
+        a <> 0 ->
+        a / b <> 0.
+      Proof. intros H1 H2. remember (Z_div_mod_eq_full a b). lia. Qed.
+
+      Hint Resolve s_positive s_nz weight_nz div_nz s_big' : arith.
+      Hint Resolve weight_0 weight_positive weight_multiples Weight.weight_multiples_full : arith.
+      Hint Resolve weight_div_nz weight_mod_quotient_zero : arith.
+
+      Lemma c_correct : Associational.eval c = c'.
+      Proof.
+        cbv [c]. rewrite eval_to_associational.
+        replace (s - c') with (s - Associational.eval [(1, c')]).
+        - apply eval_simple_encode; auto with arith. lia.
+        - f_equal. cbv [Associational.eval]. simpl. destruct c'; lia.
+      Qed.
+
+      Lemma p_nz : s - Associational.eval c <> 0.
+      Proof. rewrite c_correct. auto with arith. Qed.    
+      Hint Resolve p_nz : arith.
+
+      Local Open Scope nat_scope.
+
+      Definition reduce' from to before := dedup_weights (reduce_one s from (from / to) c before).
+      Definition carry' from to before := dedup_weights (Associational.carry from (to / from) before).
+      Definition borrow' from to before := dedup_weights (borrow from (from / to) before).
+
+      Hint Rewrite eval_reduce_one Associational.eval_carry eval_dedup_weights eval_borrow : push_eval.
+
+      Definition carry_from_position i x :=
+        carry' (weight i) (weight (i + 1)) x.
+
+      Lemma eval_carry_from_position i x :
+        Associational.eval (carry_from_position i x) = Associational.eval x.
+      Proof.
+        cbv [carry_from_position carry']. autorewrite with push_eval; auto with arith. Qed.
+      Hint Rewrite eval_carry_from_position : push_eval.
+
+      Definition carry_reduce i x :=
+        let x := carry_from_position (i + n) x in
+        let x := reduce' (weight (i + n)) (weight i) x in
+        carry_from_position i x.
+
+      Lemma eval_carry_reduce i x :
+        (Associational.eval (carry_reduce i x) mod (s - Associational.eval c) =
+           Associational.eval x mod (s - Associational.eval c))%Z.
+      Proof. cbv [carry_reduce reduce']. autorewrite with push_eval; auto with arith. Qed.
+      Hint Rewrite eval_carry_reduce : push_eval.
+
+      (* rw stands for "register_width".
+         The idea here is that, if x has value 0 at weight (i + n + 1), then
+         carry_reduce_rw i x = carry_reduce (i + 1) (carry_reduce i x).
+
+         The benefit of using carry_reduce_rw, then, instead of a couple of carry_reduces,
+         is that (in C, or something similar), the LHS of the equation above takes less work
+         to calculate than the RHS.  This is because carries by 2^register_width are very easy.
+       *)
+      Definition carry_reduce_rw i x :=
+        let x := carry' (weight (i + n)) (weight (i + n) * 2^register_width) x in
+        let x := reduce' (weight (i + n)) (weight i) x in
+        let x := carry_from_position i x in
+        let x := reduce' (weight (i + n) * 2^register_width) (weight (i + 1)) x in
+        carry_from_position (i + 1) x.
+
+      Local Open Scope Z_scope.
+
+      Lemma reduction_divides i : weight (n + i - 1) * 2^register_width / weight i mod s = 0.
+      Proof.
+        rewrite Divide.Z.mod_divide_full. apply (Z.divide_trans _ (weight (n + i) / weight i)).
+        - rewrite <- Divide.Z.mod_divide_full. rewrite (Nat.add_comm n i). apply s_small.
+        - apply Z.divide_div.
+          + remember (weight_positive i). lia.
+          + rewrite <- Divide.Z.mod_divide_full. apply Weight.weight_multiples_full; try assumption.
+            lia.
+          + rewrite <- Divide.Z.mod_divide_full.
+            replace (weight (n + i)) with (weight (n + i - 1 + 1)).
+            -- apply weight_lt_width.
+            -- f_equal. lia.
+      Qed.
+
+      Lemma reduction_divides' (i j : nat) :
+        (j = n + i - 1)%nat ->
+        weight j * 2^register_width / weight i mod s = 0.
+      Proof. intros H. subst. apply reduction_divides. Qed.
+
+      Lemma weight_prod_mod_zero (i j : nat) :
         (i <= j)%nat ->
-        (weight j) mod (weight j / weight i) = 0.
-    Proof.
-      intros i j H. apply mod_quotient_zero; try apply weight_positive.
-      apply Weight.weight_multiples_full; assumption.
-    Qed.
+        (weight j * 2^register_width) mod (weight i) = 0.
+      Proof.
+        intros H. apply Divide.Z.mod_divide_full. apply Z.divide_mul_l.
+        rewrite <- Divide.Z.mod_divide_full. apply Weight.weight_multiples_full; try assumption.
+      Qed.
 
-    Lemma divisible_implies_nonzero a b : 
-      a mod b = 0 ->
-      a <> 0 ->
-      a / b <> 0.
-    Proof. intros H1 H2. remember (Z_div_mod_eq_full a b). lia. Qed.
+      Lemma weight_prod_div_nz (i j : nat) :
+        (i <= j)%nat ->
+        weight j * 2^register_width / weight i <> 0.
+      Proof.
+        intros H. apply divisible_implies_nonzero. apply weight_prod_mod_zero; try lia.
+        remember (weight_positive j). remember (Z.pow_nonneg 2 register_width). lia.
+      Qed.
 
-    Hint Resolve s_positive s_nz weight_nz div_nz s_big' : arith.
-    Hint Resolve weight_0 weight_positive weight_multiples Weight.weight_multiples_full : arith.
-    Hint Resolve weight_div_nz weight_mod_quotient_zero : arith.
+      Lemma s_small_particular : weight n mod s = 0.
+      Proof.
+        replace (weight n) with (weight n / weight 0).
+        - apply s_small'; lia.
+        - Z.div_mod_to_equations. lia.
+      Qed.
 
-    Lemma c_correct : Associational.eval c = c'.
-    Proof.
-      cbv [c]. rewrite eval_to_associational.
-      replace (s - c') with (s - Associational.eval [(1, c')]).
-      - apply eval_simple_encode; auto with arith. lia.
-      - f_equal. cbv [Associational.eval]. simpl. destruct c'; lia.
-    Qed.
-    
-    Lemma p_nz : s - Associational.eval c <> 0.
-    Proof. rewrite c_correct. auto with arith. Qed.    
-    Hint Resolve p_nz : arith.
-    
-    Local Open Scope nat_scope.
+      Lemma eval_carry_reduce_rw i x :
+        (Associational.eval (carry_reduce_rw i x) mod (s - Associational.eval c) =
+           Associational.eval x mod (s - Associational.eval c))%Z.
+      Proof.
+        cbv [carry_reduce_rw carry' reduce']. autorewrite with push_eval; auto with arith.
+        - apply weight_prod_div_nz; lia.
+        - apply weight_prod_div_nz; lia.
+        - apply mod_quotient_zero; auto with arith. apply weight_prod_mod_zero; lia.
+        - apply reduction_divides'; lia.
+      Qed.
+      Hint Rewrite eval_carry_reduce_rw : push_eval.
 
-    Definition reduce' from to before := dedup_weights (reduce_one s from (from / to) c before).
-    Definition carry' from to before := dedup_weights (Associational.carry from (to / from) before).
-    Definition borrow' from to before := dedup_weights (borrow from (from / to) before).
+      Definition carry_chain idxs x :=
+        fold_right carry_from_position x (rev idxs).
 
-    Hint Rewrite eval_reduce_one Associational.eval_carry eval_dedup_weights eval_borrow : push_eval.
+      Lemma eval_carry_chain idxs x :
+        Associational.eval (carry_chain idxs x) = Associational.eval x.
+      Proof.
+        cbv [carry_chain]. induction (rev idxs).
+        - reflexivity.
+        - simpl. autorewrite with push_eval. assumption.
+      Qed.
+      Hint Rewrite eval_carry_chain : push_eval.
 
-    Definition carry_from_position i x :=
-      carry' (weight i) (weight (i + 1)) x.
+      Definition carry_reduce_chain idxs x :=
+        fold_right carry_reduce x (rev idxs).
 
-    Lemma eval_carry_from_position i x :
-      Associational.eval (carry_from_position i x) = Associational.eval x.
-    Proof.
-      cbv [carry_from_position carry']. autorewrite with push_eval; auto with arith. Qed.
-    Hint Rewrite eval_carry_from_position : push_eval.
+      Lemma eval_carry_reduce_chain idxs x :
+        ((Associational.eval (carry_reduce_chain idxs x)) mod (s - Associational.eval c) = (Associational.eval x) mod (s - Associational.eval c))%Z.
+      Proof.
+        cbv [carry_reduce_chain]. induction (rev idxs).
+        - reflexivity.
+        - simpl. autorewrite with push_eval. assumption.
+      Qed.
+      Hint Rewrite eval_carry_reduce_chain : push_eval.
 
-    Definition carry_reduce i x :=
-      let x := carry_from_position (i + n) x in
-      let x := reduce' (weight (i + n)) (weight i) x in
-      carry_from_position i x.
+      Hint Resolve s_small_particular divisible_implies_nonzero Z_mod_same_full : arith.
 
-    Lemma eval_carry_reduce i x :
-      (Associational.eval (carry_reduce i x) mod (s - Associational.eval c) =
-      Associational.eval x mod (s - Associational.eval c))%Z.
-    Proof. cbv [carry_reduce reduce']. autorewrite with push_eval; auto with arith. Qed.
-    Hint Rewrite eval_carry_reduce : push_eval.
-
-    (* rw stands for "register_width".
-       The idea here is that, if x has value 0 at weight (i + n + 1), then
-       carry_reduce_rw i x = carry_reduce (i + 1) (carry_reduce i x).
-
-       The benefit of using carry_reduce_rw, then, instead of a couple of carry_reduces,
-       is that (in C, or something similar), the LHS of the equation above takes less work
-       to calculate than the RHS.  This is because carries by 2^register_width are very easy.
-     *)
-    Definition carry_reduce_rw i x :=
-      let x := carry' (weight (i + n)) (weight (i + n) * 2^register_width) x in
-      let x := reduce' (weight (i + n)) (weight i) x in
-      let x := carry_from_position i x in
-      let x := reduce' (weight (i + n) * 2^register_width) (weight (i + 1)) x in
-      carry_from_position (i + 1) x.
-
-    Local Open Scope Z_scope.
-
-    Lemma reduction_divides i : weight (n + i - 1) * 2^register_width / weight i mod s = 0.
-    Proof.
-      rewrite Divide.Z.mod_divide_full. apply (Z.divide_trans _ (weight (n + i) / weight i)).
-      - rewrite <- Divide.Z.mod_divide_full. rewrite (Nat.add_comm n i). apply s_small.
-      - apply Z.divide_div.
-        + remember (weight_positive i). lia.
-        + rewrite <- Divide.Z.mod_divide_full. apply Weight.weight_multiples_full; try assumption.
-          lia.
-        + rewrite <- Divide.Z.mod_divide_full.
-          replace (weight (n + i)) with (weight (n + i - 1 + 1)).
-          -- apply weight_lt_width.
-          -- f_equal. lia.
-    Qed.
-
-    Lemma reduction_divides' (i j : nat) :
-      (j = n + i - 1)%nat ->
-      weight j * 2^register_width / weight i mod s = 0.
-    Proof. intros H. subst. apply reduction_divides. Qed.
-
-    Lemma weight_prod_mod_zero (i j : nat) :
-      (i <= j)%nat ->
-      (weight j * 2^register_width) mod (weight i) = 0.
-    Proof.
-      intros H. apply Divide.Z.mod_divide_full. apply Z.divide_mul_l.
-      rewrite <- Divide.Z.mod_divide_full. apply Weight.weight_multiples_full; try assumption.
-    Qed.
-    
-    Lemma weight_prod_div_nz (i j : nat) :
-      (i <= j)%nat ->
-      weight j * 2^register_width / weight i <> 0.
-    Proof.
-      intros H. apply divisible_implies_nonzero. apply weight_prod_mod_zero; try lia.
-      remember (weight_positive j). remember (Z.pow_nonneg 2 register_width). lia.
-    Qed.
-
-    Lemma s_small_particular : weight n mod s = 0.
-    Proof.
-      replace (weight n) with (weight n / weight 0).
-      - apply s_small'; lia.
-      - Z.div_mod_to_equations. lia.
-    Qed.
-
-    Lemma eval_carry_reduce_rw i x :
-      (Associational.eval (carry_reduce_rw i x) mod (s - Associational.eval c) =
-         Associational.eval x mod (s - Associational.eval c))%Z.
-    Proof.
-      cbv [carry_reduce_rw carry' reduce']. autorewrite with push_eval; auto with arith.
-      - apply weight_prod_div_nz; lia.
-      - apply weight_prod_div_nz; lia.
-      - apply mod_quotient_zero; auto with arith. apply weight_prod_mod_zero; lia.
-      - apply reduction_divides'; lia.
-    Qed.
-    Hint Rewrite eval_carry_reduce_rw : push_eval.
-
-    Definition carry_chain idxs x :=
-      fold_right carry_from_position x (rev idxs).
-
-    Lemma eval_carry_chain idxs x :
-      Associational.eval (carry_chain idxs x) = Associational.eval x.
-    Proof.
-      cbv [carry_chain]. induction (rev idxs).
-      - reflexivity.
-      - simpl. autorewrite with push_eval. assumption.
-    Qed.
-    Hint Rewrite eval_carry_chain : push_eval.
-    
-    Definition carry_reduce_chain idxs x :=
-      fold_right carry_reduce x (rev idxs).
-      
-    Lemma eval_carry_reduce_chain idxs x :
-      ((Associational.eval (carry_reduce_chain idxs x)) mod (s - Associational.eval c) = (Associational.eval x) mod (s - Associational.eval c))%Z.
-    Proof.
-      cbv [carry_reduce_chain]. induction (rev idxs).
-      - reflexivity.
-      - simpl. autorewrite with push_eval. assumption.
-    Qed.
-    Hint Rewrite eval_carry_reduce_chain : push_eval.
-
-    Hint Resolve s_small_particular divisible_implies_nonzero Z_mod_same_full : arith.
-
-    (* combine the values at position (n - 1) and n;
-       then, split the combined value into
-       pieces at position (n - 1) and weight s.
-     *)
-    Definition move_to_weight_s x :=
-      let x := carry' (weight (n - 1)) s x in
-      borrow' (weight n) s x.
-
-    Lemma eval_move_to_weight_s x :
-      Associational.eval (move_to_weight_s x) = Associational.eval x.
-    Proof.
-      cbv [move_to_weight_s borrow' carry']. autorewrite with push_eval; auto with arith.
-      apply mod_quotient_zero; auto with arith. remember s_positive. lia.
-    Qed.
-    Hint Rewrite eval_move_to_weight_s : push_eval.
-
-    (* This function is a reduction from position n to position 0---
-       the main idea is to do something like 'let x := carry_reduce 0 x'.
-
-       In fact, we move everything from position n to weight s, as well
-       as taking the top few bits off position (n - 1) to put them in weight s,
-       before doing the reduction from weight s to position 0.
-
-       This gives us the opportunity to reduce from the top of position (n - 1),
-       as well as from position n, while only having to do one reduction.
-     *)
-    Definition carry_reduce_s x :=
-      let x := carry_from_position n x in
-      let x := move_to_weight_s x in
-      let x := reduce' s (weight 0) x in
-      carry_from_position 0 x.
-
-    Lemma eval_carry_reduce_s x :
-      ((Associational.eval (carry_reduce_s x)) mod (s - Associational.eval c) =
-      (Associational.eval x) mod (s - Associational.eval c))%Z.
-    Proof.
-      cbv [carry_reduce_s reduce']. autorewrite with push_eval; auto with arith.
-      - rewrite weight_0. rewrite Z.div_1_r. apply s_nz.
-      - rewrite weight_0. rewrite Z.div_1_r. auto with arith.
-      - rewrite weight_0. rewrite Z.div_1_r. auto with arith.
-    Qed.
-    Hint Rewrite eval_carry_reduce_s : push_eval.
-
-    Local Open Scope nat_scope.
-
-    Definition seq_from_to a b := seq a (Z.to_nat (b - a + 1)).
-
-    (* The main idea here is to have something like this:
-           Definition overly_simple_reduce_carry_borrow x :=
-                      carry_reduce_chain (seq_from_to 0 (n - 1)) x.
-       Below, we have something like this, with a few extra things added in.
-     *)
-    Definition reduce_carry_borrow x :=
-      let x := dedup_weights x in
-
-      (* In the 'overly_simple_reduce_carry_borrow', the following code block
-         would belong in the position marked with an 'A' down below.
-         It turns out that doing that might make the output bounds too loose.
-
-         In particular, we need last_reduction to be small enough so that the final
-         carry chain (right below the 'A') does not overflow position (n - 1).
-         We solve this issue by putting the code block here (instad of at 'A').
-
-         This way, the reductions that land in positions
-              last_reduction + 1, last_reduction + 2, ..., n - 2, n - 1
-         are carried up to position n (before the reduction from position n),
-         so we don't have to worry about them overflowing position (n - 1).
-
-         Note that, other than this constraint requiring last_reduction to be
-         sufficiently small, we want to choose the last_reduction parameter to
-         be as large as possible, since when it gets smaller, the final carry
-         chain gets longer (and everything else takes the same amount of time).
+      (* combine the values at position (n - 1) and n;
+         then, split the combined value into
+         pieces at position (n - 1) and weight s.
        *)
-      let x := carry_reduce_chain (seq_from_to (last_reduction + 1) (n - 3)) x in
-      let x := carry_reduce_rw (n - 2) x in
+      Definition move_to_weight_s x :=
+        let x := carry' (weight (n - 1)) s x in
+        borrow' (weight n) s x.
 
-      (* This next code block is similar to writing
-              let x := carry_reduce 0 x,
-         except it's a bit more clever.
-         While reducing from position n to position 0, we simultaneously reduce
-         the top few bits of position (n - 1) down to position 0.
+      Lemma eval_move_to_weight_s x :
+        Associational.eval (move_to_weight_s x) = Associational.eval x.
+      Proof.
+        cbv [move_to_weight_s borrow' carry']. autorewrite with push_eval; auto with arith.
+        apply mod_quotient_zero; auto with arith. remember s_positive. lia.
+      Qed.
+      Hint Rewrite eval_move_to_weight_s : push_eval.
+
+      (* This function is a reduction from position n to position 0---
+         the main idea is to do something like 'let x := carry_reduce 0 x'.
+
+         In fact, we move everything from position n to weight s, as well
+         as taking the top few bits off position (n - 1) to put them in weight s,
+         before doing the reduction from weight s to position 0.
+
+         This gives us the opportunity to reduce from the top of position (n - 1),
+         as well as from position n, while only having to do one reduction.
        *)
-      let x := carry_reduce_s x in
+      Definition carry_reduce_s x :=
+        let x := carry_from_position n x in
+        let x := move_to_weight_s x in
+        let x := reduce' s (weight 0) x in
+        carry_from_position 0 x.
 
-      (* This code block is what remains (after we've finished adding in all the
-         extra stuff) of the 'overly_simple_reduce_carry_borrow' referred to above.
+      Lemma eval_carry_reduce_s x :
+        ((Associational.eval (carry_reduce_s x)) mod (s - Associational.eval c) =
+           (Associational.eval x) mod (s - Associational.eval c))%Z.
+      Proof.
+        cbv [carry_reduce_s reduce']. autorewrite with push_eval; auto with arith.
+        - rewrite weight_0. rewrite Z.div_1_r. apply s_nz.
+        - rewrite weight_0. rewrite Z.div_1_r. auto with arith.
+        - rewrite weight_0. rewrite Z.div_1_r. auto with arith.
+      Qed.
+      Hint Rewrite eval_carry_reduce_s : push_eval.
 
-         The only clever part is that the last two carry_reduces have been replaced
-         with a carry_reduce_rw.
+      Local Open Scope nat_scope.
+
+      Definition seq_from_to a b := seq a (Z.to_nat (b - a + 1)).
+
+      (* The main idea here is to have something like this:
+             Definition overly_simple_reduce_carry_borrow x :=
+                        carry_reduce_chain (seq_from_to 0 (n - 1)) x.
+         Below, we have something like this, with a few extra things added in.
        *)
-      let x := carry_reduce_chain (seq_from_to 1 (last_reduction - 1)) x in
-      let x := carry_reduce_rw last_reduction x in
+      Definition reduce_carry_borrow x :=
+        let x := dedup_weights x in
 
-      (* A *)
+        (* In the 'overly_simple_reduce_carry_borrow', the following code block
+           would belong in the position marked with an 'A' down below.
+           It turns out that doing that might make the output bounds too loose.
 
-      let x := carry_chain (seq_from_to (last_reduction + 2) (n - 2)) x in
+           In particular, we need last_reduction to be small enough so that the final
+           carry chain (right below the 'A') does not overflow position (n - 1).
+           We solve this issue by putting the code block here (instad of at 'A').
 
-      Positional.from_associational weight n x.
+           This way, the reductions that land in positions
+                  last_reduction + 1, last_reduction + 2, ..., n - 2, n - 1
+           are carried up to position n (before the reduction from position n),
+           so we don't have to worry about them overflowing position (n - 1).
 
-    Definition mulmod a b :=
-      let a_assoc := Positional.to_associational weight n a in
-      let b_assoc := Positional.to_associational weight n b in
-      let x := Associational.mul a_assoc b_assoc in
-      reduce_carry_borrow x.
+           Note that, other than this constraint requiring last_reduction to be
+           sufficiently small, we want to choose the last_reduction parameter to
+           be as large as possible, since when it gets smaller, the final carry
+           chain gets longer (and everything else takes the same amount of time).
+         *)
+        let x := carry_reduce_chain (seq_from_to (last_reduction + 1) (n - 3)) x in
+        let x := carry_reduce_rw (n - 2) x in
 
-    Definition squaremod a :=
-      let a_assoc := Positional.to_associational weight n a in
-      let x := Associational.square a_assoc in
-      reduce_carry_borrow x.
+        (* This next code block is similar to writing
+                let x := carry_reduce 0 x,
+           except it's a bit more clever.
+           While reducing from position n to position 0, we simultaneously reduce
+           the top few bits of position (n - 1) down to position 0.
+         *)
+        let x := carry_reduce_s x in
 
-    Hint Rewrite Positional.eval_from_associational Positional.eval_to_associational : push_eval.
+        (* This code block is what remains (after we've finished adding in all the
+           extra stuff) of the 'overly_simple_reduce_carry_borrow' referred to above.
 
-    Local Open Scope Z_scope.
-      
-    Lemma eval_reduce_carry_borrow r0 :
-      (Positional.eval weight n (reduce_carry_borrow r0)) mod (s - Associational.eval c) =
-      (Associational.eval r0) mod (s - Associational.eval c).
-    Proof.
-      cbv [reduce_carry_borrow carry' reduce' borrow'].
-      autorewrite with push_eval; auto with arith; try lia.
-    Qed.
-    Hint Rewrite eval_reduce_carry_borrow : push_eval.
+           The only clever part is that the last two carry_reduces have been replaced
+           with a carry_reduce_rw.
+         *)
+        let x := carry_reduce_chain (seq_from_to 1 (last_reduction - 1)) x in
+        let x := carry_reduce_rw last_reduction x in
 
-    Theorem eval_mulmod a b :
-      (Positional.eval weight n (mulmod a b)) mod (s - c') =
-      (Positional.eval weight n a * Positional.eval weight n b) mod (s - c').
-    Proof.
-      cbv [mulmod]. rewrite <- c_correct. autorewrite with push_eval. reflexivity.
-    Qed.
+        (* A *)
 
-    Theorem eval_squaremod a :
-      (Positional.eval weight n (squaremod a)) mod (s - c') =
-      (Positional.eval weight n a * Positional.eval weight n a) mod (s - c').
-    Proof.
-      cbv [squaremod]. rewrite <- c_correct. autorewrite with push_eval. reflexivity.
-    Qed.
-  End DettmanMultiplication.
+        let x := carry_chain (seq_from_to (last_reduction + 2) (n - 2)) x in
+
+        Positional.from_associational weight n x.
+
+      Definition mulmod a b :=
+        let a_assoc := Positional.to_associational weight n a in
+        let b_assoc := Positional.to_associational weight n b in
+        let x := Associational.mul a_assoc b_assoc in
+        reduce_carry_borrow x.
+
+      Definition squaremod a :=
+        let a_assoc := Positional.to_associational weight n a in
+        let x := Associational.square a_assoc in
+        reduce_carry_borrow x.
+
+      Hint Rewrite Positional.eval_from_associational Positional.eval_to_associational : push_eval.
+
+      Local Open Scope Z_scope.
+
+      Lemma eval_reduce_carry_borrow r0 :
+        (Positional.eval weight n (reduce_carry_borrow r0)) mod (s - Associational.eval c) =
+          (Associational.eval r0) mod (s - Associational.eval c).
+      Proof.
+        cbv [reduce_carry_borrow carry' reduce' borrow'].
+        autorewrite with push_eval; auto with arith; try lia.
+      Qed.
+      Hint Rewrite eval_reduce_carry_borrow : push_eval.
+
+      Theorem eval_mulmod a b :
+        (Positional.eval weight n (mulmod a b)) mod (s - c') =
+          (Positional.eval weight n a * Positional.eval weight n b) mod (s - c').
+      Proof.
+        cbv [mulmod]. rewrite <- c_correct. autorewrite with push_eval. reflexivity.
+      Qed.
+
+      Theorem eval_squaremod a :
+        (Positional.eval weight n (squaremod a)) mod (s - c') =
+          (Positional.eval weight n a * Positional.eval weight n a) mod (s - c').
+      Proof.
+        cbv [squaremod]. rewrite <- c_correct. autorewrite with push_eval. reflexivity.
+      Qed.
+    End WithoutADK.
+
+    Section WithADK.
+      Import pmul.
+      (* now we'll add the option to use the adk algorithm in place of associational.mul *)
+      Context (weight_friendly : forall i j : nat, weight i * weight j = weight (i + j)).
+
+      (*Definition ZZ_is_bounded_by_bool (x : Z) (bounds : Z*Z) : bool :=
+        (fst bounds <=? x) && (x <=? snd bounds).
+    
+      Definition is_bounded_by (l : list Z) (bounds : list (Z*Z)) : bool :=
+        fold_right andb true
+          (map (fun x_bound => ZZ_is_bounded_by_bool (fst x_bound) (snd x_bound))
+             (combine l bounds)).
+
+      Definition is_lower_bounded_by (bounds : list (Z*Z)) (xs : list Z) : bool :=
+        fold_right andb true
+          (map (fun bound_x => snd bound_x <=? fst (fst bound_x))
+             (combine bounds xs)).
+
+      (* if everything is nonnegative, then the output is nondecreasing in the inputs *)
+      Definition output_bounds (n : nat) (x_bounds y_bounds : list (Z*Z)) : list (Z*Z) :=
+        let lower_bounds := adk_mul n (map fst x_bounds) (map fst y_bounds) in
+        let upper_bounds := adk_mul n (map snd x_bounds) (map snd y_bounds) in
+        map (fun lower_upper => (fst lower_upper, snd lower_upper))
+          (combine lower_bounds upper_bounds).
+
+      Definition list_if_then_else {X} (cond : bool) (ifval elseval : list X) : list X :=
+        map (fun if_else => if cond then fst if_else else snd if_else) (combine ifval elseval).
+
+      Lemma list_if_then_else_spec {X} (cond : bool) (ifval elseval : list X) :
+        let len := Nat.min (length ifval) (length elseval) in
+        list_if_then_else cond ifval elseval =
+          if cond then (firstn len ifval) else (firstn len elseval).
+      Proof.
+        cbv [list_if_then_else]. destruct (length ifval <=? length elseval)%nat eqn:E.
+        - apply Nat.leb_le in E.
+          replace (Nat.min (length ifval) (length elseval)) with (length ifval) by lia.
+          destruct cond.
+          + rewrite firstn_all. rewrite <- (@firstn_all2 _ (length elseval)) by lia.
+            apply ListUtil.map_fst_combine. (* wow, eta reduction *)
+          + apply ListUtil.map_snd_combine.
+        - apply Nat.leb_nle in E.
+          replace (Nat.min (length ifval) (length elseval)) with (length elseval) by lia.
+          destruct cond.
+          + apply ListUtil.map_fst_combine.
+          + rewrite firstn_all. rewrite <- (@firstn_all2 _ (length ifval)) by lia.
+            apply ListUtil.map_snd_combine.
+      Qed.
+
+      Definition truncate (values : list Z) (upper_bounds : list Z) :=
+        map (fun x_upper => Z.land (fst x_upper) (Z.ones (Z.log2_up (snd x_upper)))) (combine values upper_bounds).
+    
+      Definition adk_mul_with_bounds (x_bounds y_bounds : list (Z*Z)) (x y : list Z) : list Z :=
+        list_if_then_else
+          (is_lower_bounded_by x_bounds (repeat 0 n) &&
+           is_lower_bounded_by y_bounds (repeat 0 n) &&
+           ZZ_is_bounded_by_bool (pmul.nth_reifiable 0 x 0) (pmul.nth_reifiable 0 x_bounds (0, 0)) &&
+           is_bounded_by y y_bounds)
+          (truncate (adk_mul n x y)
+             (map snd (output_bounds n x_bounds y_bounds)))
+          (pmul.pmul n x y). Print adk_mul.*)
+
+      Definition adk_mulmod (*(x_bounds y_bounds : list (Z*Z))*) (x y : list Z) : list Z :=
+        reduce_carry_borrow (Positional.to_associational weight n (adk_mul (*_with_bounds x_bounds y_bounds*) n x y)).
+
+      Theorem eval_adk_mulmod (*a_bounds b_bounds*) a b :
+        (Positional.eval weight n (adk_mulmod (*a_bounds b_bounds*) a b)) mod (s - c') =
+          (Positional.eval weight n a * Positional.eval weight n b) mod (s - c').
+      Proof.
+        cbv [adk_mulmod]. rewrite <- c_correct. rewrite eval_reduce_carry_borrow.
+        - Search to_associational. rewrite eval_to_associational. f_equal. 
+          Check eval_reduce_carry_borrow. Search adk_mul.
+      Admitted. Check adk_mulmod.
+    End WithADK.
+  End DettmanMultiplication.  
 End DettmanMultiplication.
+(*Require Import Crypto.BoundsPipeline.
+      Print Reify.
+Import
+  AbstractInterpretation.Compilers
+  Language.Compilers
+  Language.API.Compilers.
+
+Import Language.API.Compilers.API.
+Import pmul.
+Import DettmanMultiplication.
+Locate "Reify".
+Check adk_mulmod.
+Print pmul.adk_mul'.
+Print adk_mul_prod_at_i. Print nth_reifiable. Check adk_mulmod.
+Print adk_mulmod. Check reduce_carry_borrow. Print reduce_carry_borrow.
+Compute (ltac: (let r := Reify (adk_mulmod)
+                            in
+                  exact r)).*)
+
+(*Definition nn := 5%nat.
+      Definition xx := [543; 654; 234; 123; 5698].
+      Definition yy := [890423; 432; 321; 1; 232].
+      Definition weightt i := 2^i.
+      Compute (dedup_weights (DettmanMultiplication.adk_mul' nn weightt xx yy)).
+      Compute (dedup_weights (Associational.mul (Positional.to_associational weightt nn xx)
+                                                (Positional.to_associational weightt nn yy))).*)
 
 Module dettman_multiplication_mod_ops.
   Section dettman_multiplication_mod_ops.
@@ -413,9 +519,9 @@ Module dettman_multiplication_mod_ops.
     (* I don't want these to be automatically unfolded in the proofs below. *)
     Definition limbwidth_num := limbwidth_num'.
     Definition limbwidth_den := limbwidth_den'.
-    
+
     Definition weight := (weight limbwidth_num limbwidth_den).
-    
+
     Definition mulmod := mulmod s c register_width n last_reduction weight.
     Definition squaremod := squaremod s c register_width n last_reduction weight.
 
@@ -547,15 +653,61 @@ Module dettman_multiplication_mod_ops.
         + replace 0%Q with (inject_Z 0) by reflexivity. rewrite <- Zle_Qle. lia.
     Qed.
 
-    Definition eval_mulmod := eval_mulmod s c register_width n last_reduction weight p_nz n_gteq_4 s_small s_big weight_lt_width wprops.
-    Definition eval_squaremod := eval_squaremod s c register_width n last_reduction weight p_nz n_gteq_4 s_small s_big weight_lt_width wprops.
+    Definition eval_mulmod := eval_mulmod s c register_width n last_reduction weight p_nz n_gteq_4 wprops s_small s_big weight_lt_width.
+    Definition eval_squaremod := eval_squaremod s c register_width n last_reduction weight p_nz n_gteq_4 wprops s_small s_big weight_lt_width.
   End dettman_multiplication_mod_ops.
 End dettman_multiplication_mod_ops.
 
+Module dettman_multiplication_with_adk_mod_ops.
+  Section dettman_multiplication_with_adk_mod_ops.
+    Import DettmanMultiplication.
+    Local Open Scope Z_scope.
+    Context
+        (s : Z)
+        (c : Z)
+        (register_width : nat)
+        (n : nat)
+        (limbwidth : nat)
+        (last_reduction : nat)
+        (p_nz : s - c <> 0)
+        (n_gteq_4 : (4 <= n)%nat)
+        (limbwidth_nz : 0 <> limbwidth)
+        (s_power_of_2 : 2 ^ (Z.log2 s) = s)
+        (s_big' : (n - 1) * limbwidth <= Z.log2 s)
+        (s_small' : Z.log2 s <= n * limbwidth)
+        (registers_big : limbwidth <= register_width).
+
+    Definition weight := weight limbwidth 1.
+
+    Lemma limbwidth_good : 0 < 1 <= limbwidth.
+    Proof. remember limbwidth_nz. lia. Qed.
+    Local Notation wprops := (@wprops limbwidth 1 limbwidth_good).
+
+    Lemma weight_simple : forall i, weight i = 2 ^ (i * limbwidth).
+    Proof.
+      intros i. rewrite (ModOps.weight_ZQ_correct _ _ limbwidth_good).
+      cbv [Qdiv]. replace (Qinv (inject_Z 1)) with 1%Q by reflexivity.
+      rewrite Qmult_1_r. rewrite <- inject_Z_mult. rewrite Qceiling_Z.
+      f_equal. lia.
+    Qed. Print adk_mulmod.
+
+    Definition adk_mulmod := adk_mulmod s c register_width n last_reduction weight.
+
+    Lemma weight_friendly : forall i j : nat, weight i * weight j = weight (i + j).
+    Proof.
+      intros i j. repeat rewrite weight_simple. rewrite <- Z.pow_add_r; try lia. f_equal. lia.
+    Qed.
+  
+    Definition eval_adk_mulmod := eval_adk_mulmod s c register_width n last_reduction weight p_nz n_gteq_4 wprops weight_friendly.
+  End dettman_multiplication_with_adk_mod_ops.
+End dettman_multiplication_with_adk_mod_ops.
 Module Export Hints.
   Import dettman_multiplication_mod_ops.
+  Import dettman_multiplication_with_adk_mod_ops.
 #[global]
   Hint Rewrite eval_mulmod using solve [ auto with zarith | congruence ] : push_eval.
 #[global]
   Hint Rewrite eval_squaremod using solve [ auto with zarith | congruence ] : push_eval.
+#[global]
+  Hint Rewrite eval_adk_mulmod using solve [ auto with zarith | congruence ] : push_eval.
 End Hints.
