src/Bedrock/Standalone/StandaloneHaskellMain.v
@@ -34,6 +34,11 @@ Module Bedrock2First.
       := main_gen ForExtraction.DettmanMultiplication.PipelineMain.
   End DettmanMultiplication.
 
+  Module DettmanMultiplicationADK.
+    Definition main : IO_unit
+      := main_gen ForExtraction.DettmanMultiplicationADK.PipelineMain.
+  End DettmanMultiplicationADK.
+
   Module SolinasReduction.
     Definition main : IO_unit
       := main_gen ForExtraction.SolinasReduction.PipelineMain.
@@ -72,6 +77,11 @@ Module Bedrock2Later.
     Definition main : IO_unit
       := main_gen ForExtraction.DettmanMultiplication.PipelineMain.
   End DettmanMultiplication.
+
+  Module DettmanMultiplicationADK.
+    Definition main : IO_unit
+      := main_gen ForExtraction.DettmanMultiplicationADK.PipelineMain.
+  End DettmanMultiplicationADK.
 
   Module SolinasReduction.
     Definition main : IO_unit
