src/ExtractionHaskell/dettman_multiplication_adk.v
@@ -1,0 +1,4 @@
+Require Import Crypto.StandaloneHaskellMain.
+
+(*Redirect "/tmp/dettman_multiplication_adk.hs"*) Recursive Extraction DettmanMultiplicationADK.main.
+(* cat /tmp/dettman_multiplication_adk.hs.out | sed -f haskell.sed  > ../../dettman_multiplication_adk.hs *)
