src/ExtractionHaskell/with_bedrock2_dettman_multiplication_adk.v
@@ -1,0 +1,5 @@
+Require Import Crypto.Bedrock.Standalone.StandaloneHaskellMain.
+Import Bedrock2Later.
+
+(*Redirect "/tmp/bedrock2_dettman_multiplication_adk.hs"*) Recursive Extraction DettmanMultiplicationADK.main.
+(* cat /tmp/bedrock2_dettman_multiplication_adk.hs.out | sed -f haskell.sed  > ../../bedrock2_dettman_multiplication_adk.hs *)
