src/ExtractionOCaml/dettman_multiplication_adk.v
@@ -1,0 +1,3 @@
+Require Import Crypto.StandaloneOCamlMain.
+
+Extraction "src/ExtractionOCaml/dettman_multiplication_adk.tmp" DettmanMultiplicationADK.main.
