src/PushButtonSynthesis/DettmanMultiplicationADK.v
@@ -1,0 +1,237 @@
+(** * Push-Button Synthesis of Dettman Multiplication *)
+Require Import Coq.Strings.String.
+Require Import Coq.micromega.Lia.
+Require Import Coq.ZArith.ZArith.
+Require Import Coq.MSets.MSetPositive.
+Require Import Coq.Lists.List.
+Require Import Coq.QArith.QArith_base Coq.QArith.Qround.
+Require Import Coq.derive.Derive.
+Require Import Crypto.Util.ErrorT.
+Require Import Crypto.Util.ListUtil.
+Require Import Crypto.Util.ListUtil.FoldBool.
+Require Import Crypto.Util.Strings.Decimal.
+Require Import Crypto.Util.Strings.Show.
+Require Import Crypto.Util.ZRange.
+Require Import Crypto.Util.ZUtil.Definitions.
+Require Import Crypto.Util.ZUtil.Zselect.
+Require Import Crypto.Util.ZUtil.Tactics.LtbToLt.
+Require Import Crypto.Util.Tactics.HasBody.
+Require Import Crypto.Util.Tactics.Head.
+Require Import Crypto.Util.Tactics.SpecializeBy.
+Require Import Rewriter.Language.Wf.
+Require Import Rewriter.Language.Language.
+Require Import Crypto.Language.API.
+Require Import Crypto.AbstractInterpretation.AbstractInterpretation.
+Require Import Crypto.Stringification.Language.
+Require Import Crypto.Arithmetic.Core.
+Require Import Crypto.Arithmetic.ModOps.
+Require Import Crypto.BoundsPipeline.
+Require Import Crypto.COperationSpecifications.
+Require Import Crypto.PushButtonSynthesis.ReificationCache.
+Require Import Crypto.PushButtonSynthesis.Primitives.
+Require Import Crypto.PushButtonSynthesis.DettmanMultiplicationADKReificationCache.
+Require Import Crypto.Arithmetic.DettmanMultiplication.
+
+Require Import Crypto.Assembly.Equivalence.
+Import ListNotations.
+Local Open Scope string_scope. Local Open Scope Z_scope. Local Open Scope list_scope. Local Open Scope bool_scope.
+
+Import
+  Language.Wf.Compilers
+  Language.Compilers
+  AbstractInterpretation.Compilers
+  Stringification.Language.Compilers.
+Import Compilers.API.
+
+Import COperationSpecifications.Primitives.
+Import COperationSpecifications.DettmanMultiplication.
+
+Import Associational Positional.
+
+Import dettman_multiplication_with_adk_mod_ops.
+
+Local Coercion Z.of_nat : nat >-> Z.
+Local Coercion QArith_base.inject_Z : Z >-> Q.
+Local Coercion Z.pos : positive >-> Z.
+
+Local Set Keyed Unification. (* needed for making [autorewrite] fast, c.f. COQBUG(https://github.com/coq/coq/issues/9283) *)
+(* needed for making [autorewrite] not take a very long time *)
+Local Opaque reified_mul_gen.
+(* needed for making [autorewrite] with [Set Keyed Unification] fast *)
+Local Opaque expr.Interp.
+
+Section __.
+  Context {output_language_api : ToString.OutputLanguageAPI}
+          {pipeline_opts : PipelineOptions}
+          {pipeline_to_string_opts : PipelineToStringOptions}
+          {synthesis_opts : SynthesisOptions}
+          (machine_wordsize : machine_wordsize_opt)
+          (s : Z)
+          (c_ : list (Z*Z))
+          (n : nat) (* number of limbs *)
+          (limbwidth : nat)
+          (last_reduction : nat)
+          (inbounds_multiplier : option Q).
+
+  Local Instance override_pipeline_opts : PipelineOptions
+    := {| widen_bytes := true (* true, because we don't allow byte-sized things anyway, so we should not expect carries to be widened to byte-size when emitting C code *)
+       |}.
+
+  (* We include [0], so that even after bounds relaxation, we can
+       notice where the constant 0s are, and remove them. *)
+  Definition possible_values_of_machine_wordsize
+    := prefix_with_carry [machine_wordsize; 2 * machine_wordsize].
+  
+  Local Notation c := (Associational.eval c_).
+  Definition m := s - c.
+
+  Local Notation possible_values := possible_values_of_machine_wordsize.
+  Definition last_limb_width : nat := (Z.to_nat (Z.log2 s)) - (n - 1) * limbwidth.
+
+  Definition input_magnitude := Option.value inbounds_multiplier 1.
+  Definition output_magnitude_first_limbs : Q := input_magnitude / 2 + 1 / 2.
+  Definition output_magnitude_last_limb : Q := input_magnitude / 2 + 1 / 4.
+  (* Where these bounds came from:
+     https://github.com/bitcoin-core/secp256k1/blob/0eb3000417fcf996e3805d0eb00f0f32b8849315/src/field_5x52_impl.h#L545
+     These bounds are correct, and reasonably tight, for the following parameters:
+           s = 2^256
+           c = 2^32 - 2^9 - 2^8 - 2^7 - 2^6 - 2^4 - 1
+           n = 5
+           last_limb_width = 48
+           last_reduction = 2.
+
+           s = 2^256
+           c = 2^32 - 2^9 - 2^8 - 2^7 - 2^6 - 2^4 - 1
+           n = 10
+           last_limb_width = 22
+           last_reduction = 6.
+     Given parameters dissimilar to those above, these bounds are no better than a guess.
+     I suppose they provide a reasonable default, though. *)
+
+  Definition weightf := weight limbwidth.
+  Definition input_bounds : list (ZRange.type.option.interp base.type.Z)
+    := fold_left (fun l i => Some r[0 ~> Qceiling (2 * input_magnitude * ((weightf (i + 1) / weightf i) - 1))]%zrange :: l) (seq 0 (n - 1)) [] ++
+                 [Some r[0 ~> Qceiling (2 * input_magnitude * (2^last_limb_width - 1))]%zrange].
+  Definition output_bounds : list (ZRange.type.option.interp base.type.Z)
+    := fold_left (fun l i => Some r[0 ~> Qceiling (2 * output_magnitude_first_limbs * ((weightf (i + 1) / weightf i) - 1))]%zrange :: l) (seq 0 (n - 1)) [] ++
+         [Some r[0 ~> Qceiling (2 * output_magnitude_last_limb * (2^last_limb_width - 1))]%zrange].
+  Local Existing Instance default_translate_to_fancy.
+  Local Instance no_select_size : no_select_size_opt := no_select_size_of_no_select machine_wordsize.
+  Local Instance split_mul_to : split_mul_to_opt := split_mul_to_of_should_split_mul machine_wordsize possible_values.
+  Local Instance split_multiret_to : split_multiret_to_opt := split_multiret_to_of_should_split_multiret machine_wordsize possible_values.
+
+  (** Note: If you change the name or type signature of this
+        function, you will need to update the code in CLI.v *)
+  Definition check_args {T} (requests : list string) (res : Pipeline.ErrorT T)
+    : Pipeline.ErrorT T
+    := check_args_of_list
+         (List.map
+            (fun v => (true, v))
+            [(negb (s - c =? 0), Pipeline.Values_not_provably_distinctZ "s - c <> 0" (s - c) 0)
+             ; (4 <=? n, Pipeline.Value_not_leZ "4 <= n" 4 n)
+             ; (negb (0 =? limbwidth), Pipeline.Values_not_provably_distinctZ "0 <> limbwidth" 0 limbwidth)
+             ; (2 ^ (Z.log2 s) =? s, Pipeline.Values_not_provably_equalZ "2 ^ (Z.log2 s) = s" (2 ^ Z.log2 s) s)
+             ; ((n - 1) * limbwidth <=? Z.log2 s, Pipeline.Value_not_leZ "(n - 1) * limbwidth <= Z.log2 s" ((n - 1) * limbwidth) (Z.log2 s))
+             ; (Z.log2 s <=? n * limbwidth, Pipeline.Value_not_leZ "Z.log2 s <= n * limbwidth" (Z.log2 s) (n * limbwidth))
+             ; (limbwidth <=? machine_wordsize, Pipeline.Value_not_leZ "limbwidth <= machine_word_size" limbwidth machine_wordsize)
+            ])
+            res.
+
+  Context (requests : list string)
+    (curve_good : check_args requests (Success tt) = Success tt).
+
+  Lemma use_curve_good
+    : s - c <> 0
+      /\ (4 <= n)
+      /\ 0 <> limbwidth
+      /\ 2 ^ (Z.log2 s) = s
+      /\ (n - 1) * limbwidth <= Z.log2 s
+      /\ Z.log2 s <= n * limbwidth
+      /\ limbwidth <= machine_wordsize.
+  Proof using curve_good. prepare_use_curve_good (). Qed.
+
+  Local Notation evalf := (eval weightf n).
+  Local Notation notations_for_docstring
+    := (CorrectnessStringification.dyn_context.cons
+          weightf "weight"
+          (CorrectnessStringification.dyn_context.cons
+             evalf "eval"
+             CorrectnessStringification.dyn_context.nil))%string.
+  Local Notation "'docstring_with_summary_from_lemma!' summary correctness"
+    := (docstring_with_summary_from_lemma_with_ctx!
+          notations_for_docstring
+          summary
+          correctness)
+         (only parsing, at level 10, summary at next level, correctness at next level).
+
+  Check reified_mul_gen. Print adk_mulmod.
+
+  Definition mul
+    := Pipeline.BoundsPipeline
+         false (* subst01 *)
+         possible_values
+         (reified_mul_gen
+            @ GallinaReify.Reify s @ GallinaReify.Reify c
+            @ GallinaReify.Reify (Z.to_nat machine_wordsize) @ GallinaReify.Reify n
+            @ GallinaReify.Reify limbwidth @ GallinaReify.Reify last_reduction)
+         (Some input_bounds, (Some input_bounds, tt))
+         (Some output_bounds).
+
+
+  Definition smul (prefix : string)
+    : string * (Pipeline.M (Pipeline.ExtendedSynthesisResult _))
+    := Eval cbv beta in
+        FromPipelineToString!
+          machine_wordsize prefix "mul" mul
+          (docstring_with_summary_from_lemma!
+             (fun fname : string => [text_before_function_name ++ fname ++ " multiplies two field elements."]%string)
+             (mul_correct weightf n m input_bounds output_bounds)).
+
+  (** Work around COQBUG(https://github.com/coq/coq/issues/9286) *)
+  Local Opaque DettmanMultiplication.adk_mulmod.
+
+  Local Ltac prove_correctness _ := Primitives.prove_correctness use_curve_good.
+
+  Lemma mul_correct res
+        (Hres : mul = Success res)
+    : mul_correct (weightf) n m input_bounds output_bounds (Interp res).
+  Proof using curve_good. prove_correctness (). Qed.
+
+  Lemma Wf_mul res (Hres : mul = Success res) : Wf res.
+  Proof using Type. prove_pipeline_wf (). Qed.
+
+  Section for_stringification.
+    Local Open Scope string_scope.
+    Local Open Scope list_scope.
+
+    Definition known_functions
+      := [("mul", wrap_s smul)].
+
+    Definition valid_names : string := Eval compute in String.concat ", " (List.map (@fst _ _) known_functions).
+
+    (** Note: If you change the name or type signature of this
+          function, you will need to update the code in CLI.v *)
+    Definition Synthesize (comment_header : list string) (function_name_prefix : string) (requests : list string)
+      : list (synthesis_output_kind * string * Pipeline.M (list string))
+      := Primitives.Synthesize
+           machine_wordsize valid_names known_functions (fun _ => nil) all_typedefs!
+           check_args
+           ((ToString.comment_file_header_block
+               (comment_header
+                  ++ ["";
+                     "Computed values:";
+                     ""; ""]%string)))
+           function_name_prefix requests.
+  End for_stringification.
+End __.
+
+Module Export Hints.
+#[global]
+  Hint Opaque
+       mul
+  : wf_op_cache.
+#[global]
+  Hint Immediate
+       Wf_mul
+  : wf_op_cache.
+End Hints.
